Implement and verify decoding

src/Dafny/marshal.dfy
@@ -101,3 +101,53 @@ class {:autocontracts} Encoder
         return data;
     }
 }
+
+class {:autocontracts} Decoder
+{
+    ghost var enc: seq<Encodable>;
+    var data: array<byte>;
+    var off: nat;
+
+    predicate Valid()
+    {
+        && off <= data.Length
+        && prefix_of(seq_encode(enc), data[off..])
+    }
+
+    constructor {:autocontracts false}
+    (data: array<byte>, ghost enc: seq<Encodable>)
+    requires prefix_of(seq_encode(enc), data[..])
+    ensures Valid() && fresh(Repr - {this, data})
+    {
+        this.data := data;
+        this.off := 0;
+        this.enc := enc;
+        this.Repr := {this, data};
+    }
+
+    lemma prefix_of_app2<T>(s1: seq<T>, s2: seq<T>, n: nat)
+    requires prefix_of(s1, s2)
+    requires n <= |s1|
+    ensures prefix_of(s1[n..], s2[n..])
+    {
+    }
+
+    method DecInt(ghost x: uint64) returns (x':uint64)
+    requires |enc| > 0 && enc[0] == EncUInt64(x)
+    ensures x' == x
+    ensures enc == old(enc)[1..]
+    {
+        //assert enc == [enc[0]] + enc[1..];
+        //seq_encode_app([enc[0]], enc[1..]);
+        //assert data[off..] == data[off..off+8] + data[off+8..];
+        //assert |enc_encode(enc[0])| == 8;
+        prefix_of_app2(seq_encode(enc), data[off..], 8);
+        //assert prefix_of(seq_encode(enc[1..]), data[off+8..]);
+        x' := le_dec64(data[off..off+8]);
+        lemma_le_enc_dec64(x);
+        assert data[off..off+8] == enc_encode(EncUInt64(x));
+        off := off + 8;
+        enc := enc[1..];
+        assert Valid();
+    }
+}
